Finish inserting_two -> inserting_two case
after reverting to check_keys.
Needed to assert a total order over key_lte.

src/Key_value.thy
@@ -5,10 +5,7 @@ begin
 typedecl key
 typedecl value_t
 
-consts k_lt :: "key \<Rightarrow> key \<Rightarrow> bool"
-
-definition key_lt :: "key => key => bool" where
-  "key_lt k1 k2 == (k1 \<noteq> k2) \<and> (k_lt k1 k2)"
+consts key_lt :: "key \<Rightarrow> key \<Rightarrow> bool"
 
 definition key_le :: "key => key => bool" where
   "key_le k1 k2 == (k1 = k2) | (key_lt k1 k2)"
